proof/DDC/Language/Simple.v
@@ -1,0 +1,10 @@
+
+Require Export DDC.Language.Simple.Exp.
+Require Export DDC.Language.Simple.EsJudge.
+Require Export DDC.Language.Simple.EvJudge.
+Require Export DDC.Language.Simple.TyJudge.
+Require Export DDC.Language.Simple.SubstExpExp.
+Require Export DDC.Language.Simple.Progress.
+Require Export DDC.Language.Simple.Preservation.
+
+Require Export DDC.Language.Simple.Bonus.
