proof/Main.v
@@ -1,3 +1,4 @@
 (* Top level module imports everything so that we have a
    nice make target to build the proofs. *)
-Require Import Base.
+Require Import DDC.Base.
+Require Import DDC.Language.Simple.
